\begin{bmatrix} 0 \\ 1 \end{bmatrix} \xrightarrow{L}
\begin{bmatrix} b \\ d \end{bmatrix} \xrightarrow{L'}
L'\begin{bmatrix} b \\ d \end{bmatrix} =
\\
L'\left(b\begin{bmatrix} 1 \\ 0 \end{bmatrix} + d\begin{bmatrix} 0 \\ 1 \end{bmatrix}\right) =
\\
bL'\begin{bmatrix} 1 \\ 0 \end{bmatrix} + dL'\begin{bmatrix} 0 \\ 1 \end{bmatrix} =
\\
b\begin{bmatrix} r \\ t \end{bmatrix} + d\begin{bmatrix} s \\ u \end{bmatrix} =
\\
\begin{bmatrix} br \\ bt \end{bmatrix} + \begin{bmatrix} ds \\ du \end{bmatrix} =
\\
\begin{bmatrix} br + ds \\ bt + du \end{bmatrix}