\begin{bmatrix} 1 \\ 0 \end{bmatrix} \xrightarrow{L}
\begin{bmatrix} a \\ c \end{bmatrix} \xrightarrow{L'}
L'\begin{bmatrix} a \\ c \end{bmatrix} =
\\
L'\left(a\begin{bmatrix} 1 \\ 0 \end{bmatrix} + c\begin{bmatrix} 0 \\ 1 \end{bmatrix}\right) =
\\
aL'\begin{bmatrix} 1 \\ 0 \end{bmatrix} + cL'\begin{bmatrix} 0 \\ 1 \end{bmatrix} =
\\
a\begin{bmatrix} r \\ t \end{bmatrix} + c\begin{bmatrix} s \\ u \end{bmatrix} =
\\
\begin{bmatrix} ar \\ at \end{bmatrix} + \begin{bmatrix} cs \\ cu \end{bmatrix} =
\\
\begin{bmatrix} ar + cs \\ at + cu \end{bmatrix}