\overrightarrow{v} \times \overrightarrow{u} =\\
\begin{vmatrix}
\overrightarrow{i} & \overrightarrow{j} & \overrightarrow{k} \\
-3 & 2 & 1 \\
0 & 0 & 1
\end{vmatrix}

=\\

\overrightarrow{i}(2 \cdot 1 - 1 \cdot 0) - \overrightarrow{j}(-3 \cdot 1 - 1 \cdot 0) + \overrightarrow{k}(-3 \cdot 0 - 0 \cdot 2) =\\
\overrightarrow{i} \cdot 2 - \overrightarrow{j} \cdot -3 + \overrightarrow{k} \cdot 0 =\\
\begin{bmatrix}
2 \\ 0 \\ 0
\end{bmatrix}
-
\begin{bmatrix}
0 \\ -3 \\ 0
\end{bmatrix}
+
\begin{bmatrix}
0 \\ 0 \\ 0
\end{bmatrix}
=\\
\begin{bmatrix}
2 \\ 3 \\ 0
\end{bmatrix}